Incorporated "Code_Target_Rat" into computations

Groebner_Bases/Algorithm_Schema_Impl.thy
@@ -63,7 +63,7 @@ subsection \<open>Generating Cyclic Polynomials\<close>
 definition cycl_pp :: "nat \<Rightarrow> nat \<Rightarrow> nat \<Rightarrow> (nat \<Rightarrow>\<^sub>0 nat)"
   where "cycl_pp n d i = sparse\<^sub>0 (map (\<lambda>k. (modulo (k + i) n, 1)) [0..<d])"
 
-definition cyclic :: "nat \<Rightarrow> ((nat \<Rightarrow>\<^sub>0 nat) \<Rightarrow>\<^sub>0 rat) list"
+definition cyclic :: "nat \<Rightarrow> ((nat \<Rightarrow>\<^sub>0 nat) \<Rightarrow>\<^sub>0 'a::{zero,one,uminus}) list"
   where "cyclic n =
             (let xs = [0..<n] in
               (map (\<lambda>d. sparse\<^sub>0 (map (\<lambda>i. (cycl_pp n d i, 1)) xs)) [1..<n]) @ [sparse\<^sub>0 [(cycl_pp n n 0, 1), (0, -1)]]
