F4_Examples.thy
@@ -4,6 +4,7 @@ section \<open>Sample Computations with the F4 Algorithm\<close>
 
 theory F4_Examples
   imports F4 "Groebner_Bases/Algorithm_Schema_Impl" Jordan_Normal_Form.Gauss_Jordan_IArray_Impl
+          "Groebner_Bases/Code_Target_Rat"
 begin
 
 text \<open>We only consider scalar polynomials here, but vector-polynomials could be handled, too.\<close>
@@ -161,8 +162,8 @@ lemma
 
 end
 
-value [code] "f4_scalar_drlex (map (\<lambda>p. (p, ())) (cyclic 4)) ()"
+value [code] "length (f4_scalar_drlex (map (\<lambda>p. (p, ())) ((cyclic 4)::(_ \<Rightarrow>\<^sub>0 rat) list)) ())"
 
-value [code] "f4_scalar_drlex (map (\<lambda>p. (p, ())) (Katsura 2)) ()"
+value [code] "length (f4_scalar_drlex (map (\<lambda>p. (p, ())) (Katsura 3)) ())"
 
 end (* theory *)
