Reduced_GB_Examples.thy
@@ -1,5 +1,6 @@
 theory Reduced_GB_Examples
   imports "Groebner_Bases/Buchberger" Reduced_GB "Polynomials/MPoly_Type_Class_FMap"
+          "Groebner_Bases/Code_Target_Rat"
 begin
 
 context gd_term
